#+LATEX_CLASS: ramsay-org-article
#+LATEX_CLASS_OPTIONS: [oneside,A4paper,12pt]
#+AUTHOR: Ramsay Leung
#+EMAIL: ramsayleung@gmail.com
#+DATE: 2022-11-09 三 21:38
练习2-6:

=zero= 与 =add-1= 的定义：
#+begin_src scheme
  (define zero (lambda (f) (lambda (x) x)))

  (define (add-1 n)
    (lambda (f) (lambda (x) (f ((n f) x)))))
#+end_src

=one= 就等于将 =(add-1 zero)= 的代换结果：
#+begin_src scheme
  (lambda (f) (lambda (x) (f (((lambda (f) (lambda (x) x)) f) x))))
  ;;; =>
  (lambda (f) (lambda (x) (f ((lambda (x) x) x))))
  ;;; =>
  (lambda (f) (lambda (x) (f x)))

  ;;; one的定义：

  (lambda (f) (lambda (x) (f x)))
#+end_src

=two= 就等于将=(add-1 one)= 的代换结果：
#+begin_src scheme
  (define one (lambda (f) (lambda (x) (f x))))

  ;;; (add-1 one)
  (lambda (f) (lambda (x) (f (((lambda (f) (lambda (x) (f x))) f) x))))
  ;;; =>
  (lambda (f) (lambda (x) (f ((lambda (x) (f x)) x))))
  ;;; =>
  (lambda (f) (lambda (x) (f (f x))))
#+end_src

